Truth: improve swap-vars implementation.  Stobj-clone: fix for cloning concrete stobjs with renaming alists.

books/centaur/truth/truth.lisp
@@ -105,135 +105,376 @@
     :hints(("Goal" :in-theory (enable env-lookup)))))
 
 
-;; e.g. variable 0 initially generates 10
-;; for numvars=4, we need to generate 1010 1010  1010 1010
-;; meaning double it 3 times.  Start with n = 1.
-
-(define var-repetitions ((n natp) (val natp) (numvars natp))
-  :guard (and (<= n numvars)
-              (unsigned-byte-p (ash 1 n) val))
-  :guard-hints (("goal" :Expand ((ash 1 (+ 1 n)))
-                 :in-theory (enable logcons)))
-  :measure (nfix (- (nfix numvars) (nfix n)))
-  :returns (rep-val natp :rule-classes :type-prescription)
-  (b* ((n (lnfix n))
-       (shift (ash 1 n))
-       (val (mbe :logic (loghead shift (nfix val)) :exec val))
-       ((when (mbe :logic (zp (- (nfix numvars) n))
-                   :exec (eql n numvars)))
-        val))
-    (var-repetitions (+ 1 n)
-                     (logapp shift val val) numvars)) ///
-
-  (local (defthmd loghead-less-than-ash-gen-lemma
-           (implies (natp i)
-                    (< (loghead m x) (ash 1 (+ i (nfix m)))))
-           :hints(("Goal" :in-theory (enable* ihsext-inductions
-                                              ihsext-recursive-redefs)))))
-
-  (local (defthm loghead-less-than-ash-gen
-           (implies (<= (nfix m) (ifix n))
-                    (< (loghead m x) (ash 1 n)))
-           :hints (("goal" :use ((:instance loghead-less-than-ash-gen-lemma
-                                  (i (- (ifix n) (nfix m)))))))))
-
-  (local (defthm loghead-when-less-than-ash
-           (implies (and (< (loghead n x) (ash 1 (+ -1 n)))
-                         (posp n))
-                    (equal (loghead n x)
-                           (loghead (1- n) x)))
-           :hints(("Goal" :in-theory (enable* ihsext-inductions
-                                              ihsext-recursive-redefs)))))
-
-  (local (defthm logbitp-of-loghead-past-range
-           (implies (< (nfix n) (nfix m))
-                    (equal (logbitp n (loghead m x))
-                           (logbitp n x)))
-           :hints(("Goal" :in-theory (enable* ihsext-inductions
-                                             ihsext-recursive-redefs)))))
-
-  (local (defthmd loghead-of-plus-one
-           (implies (posp n)
-                    (equal (loghead n env)
-                           (+ (if (logbitp (1- n) env) (ash 1 (1- n)) 0)
-                              (loghead (1- n) env))))
-           :hints(("Goal" :in-theory (enable* loghead** logbitp**
-                                              ihsext-inductions)
-                   :induct t)
-                  (and stable-under-simplificationp
-                       '(:expand ((ash 1 (+ -1 n)))
-                         :in-theory (enable logcons))))))
 
 
+(local (encapsulate nil
+         (local (include-book "ihs/quotient-remainder-lemmas" :dir :system))
+         
+         (defthm mod-when-less
+           (implies (and (natp n) (natp w)
+                         (< n w))
+                    (equal (mod n w) n)))
 
-  (defret var-repetitions-invar
-    (equal (truth-eval rep-val env numvars)
-           (truth-eval (nfix val) (loghead n (nfix env)) numvars))
-    :hints(("Goal" :in-theory (enable truth-eval
-                                      bitops::logbitp-of-ash-split)
-            :induct t)
-           (and stable-under-simplificationp
-                '(:in-theory (enable loghead-of-plus-one)))))
+         (defthm mod-when-greater
+           (implies (and (natp n) (natp w)
+                         (<= w n)
+                         (syntaxp (not (equal w ''0))))
+                    (equal (mod n w)
+                           (mod (- n w) w))))
 
-  (defret var-repetitions-size
-    (implies (and (<= (nfix n) numvars)
-                  (natp numvars)
-                  (unsigned-byte-p (ash 1 (nfix n)) val))
-             (unsigned-byte-p (ash 1 numvars) rep-val))
-    :hints (("goal" :induct t
-             :expand ((ash 1 (+ 1 (nfix n))))
-             :in-theory (enable logcons))))
+         (defthm natp-of-mod
+           (implies (and (natp n) (natp w))
+                    (natp (mod n w)))
+           :hints(("Goal" :in-theory (disable (force)))))
 
-  (local (defun var-repetitions-masked-size-ind (m n val numvars)
-           (declare (xargs :measure (nfix (- (nfix numvars) (nfix n)))))
-           (b* ((n (lnfix n))
-                (shift (ash 1 n))
-                (val (mbe :logic (loghead shift (nfix val)) :exec val))
-                ((when (mbe :logic (zp (- (nfix numvars) n))
-                            :exec (eql n numvars)))
-                 (list m val)))
-             (var-repetitions-masked-size-ind
-              (+ shift m)
-              (+ 1 n)
-              (logapp shift val val)
-              numvars))))
+         (defthm mod-less-than-modulus
+           (implies (and (natp n) (posp w))
+                    (< (mod n w) w)))))
 
-  (local (defthm lognot-of-logapp
-           (equal (lognot (logapp w a b))
-                  (logapp w (lognot a) (lognot b)))
-           :hints(("Goal" :in-theory (e/d* (ihsext-inductions)
-                                           (bitops::logapp-of-i-0))
-                   :induct (logapp w a b)
-                   :expand ((:free (a b) (logapp w a b)))))))
+(local (defthm lognot-of-logapp
+         (equal (lognot (logapp w a b))
+                (logapp w (lognot a) (lognot b)))
+         :hints(("Goal" :in-theory (e/d* (ihsext-inductions)
+                                         (bitops::logapp-of-i-0))
+                 :induct (logapp w a b)
+                 :expand ((:free (a b) (logapp w a b)))))))
 
-  (local (defthm loghead-of-logapp
-           (implies (<= (nfix w1) (nfix w2))
-                    (equal (loghead w2 (logapp w1 a b))
-                           (logapp w1 a (loghead (- (nfix w2) (nfix w1)) b))))
-           :hints ((bitops::logbitp-reasoning))))
 
-  (local (defthm unsigned-byte-p-implies-width-natp
-           (implies (unsigned-byte-p n x)
-                    (natp n))
+;; BOZO consider moving this to shareable book
+(define logrepeat ((times natp) (width natp) (data integerp))
+  :returns (reps natp :rule-classes :type-prescription)
+  (if (zp times)
+      0
+    (logapp width data (logrepeat (1- times) width data)))
+  ///
+  (local (defret size-of-logrepeat-lemma
+           (unsigned-byte-p (* (nfix width) (nfix times)) reps)))
+
+  (defret size-of-logrepeat
+    (implies (and (<= (* (nfix width) (nfix times)) n)
+                  (natp n))
+             (unsigned-byte-p n reps)))
+
+  (local (defthm unsigned-byte-p-implies-natp-width
+           (implies (unsigned-byte-p m data)
+                    (natp m))
            :hints(("Goal" :in-theory (enable unsigned-byte-p)))
            :rule-classes :forward-chaining))
 
-  (local (defthm plus-minus-*-n
-           (implies (and (syntaxp (quotep n))
-                         (natp n))
-                    (equal (+ (- x) (* n x))
-                           (* (+ -1 n) x)))))
+  (local (defret size-of-logrepeat-by-data-size-lemma
+           (implies (and (unsigned-byte-p m (loghead width data))
+                         (<= m (nfix width))
+                         (posp times))
+                    (unsigned-byte-p (+ m (- (nfix width))
+                                        (* (nfix width) (nfix times)))
+                                     reps))
+           :hints (("goal" :induct <call>
+                    :expand ((:free (data) <call>))))))
 
-  (defret var-repetitions-negated-masked-size
-    (implies (and (<= (nfix n) numvars)
-                  (natp numvars)
-                  (unsigned-byte-p m (loghead (ash 1 (nfix n)) (lognot (nfix val)))))
-             (unsigned-byte-p (- (ash 1 numvars) (- (ash 1 (nfix n)) m))
-                              (loghead (ash 1 numvars) (lognot rep-val))))
-    :hints (("goal" :induct (var-repetitions-masked-size-ind m n val numvars)
-             :expand ((ash 1 (+ 1 (nfix n)))
-                      (var-repetitions n val numvars))
-             :in-theory (enable logcons)))))
+  (defret size-of-logrepeat-by-data-size
+    (implies (and (unsigned-byte-p m (loghead width data))
+                  (<= (+ m (- (nfix width))
+                         (* (nfix width) (nfix times))) n)
+                  (<= m (nfix width))
+                  (natp n))
+             (unsigned-byte-p n reps))
+    :hints (("goal" :use ((:instance size-of-logrepeat-by-data-size-lemma))
+             :in-theory (disable size-of-logrepeat-by-data-size-lemma))))
+
+  (local (defun logbitp-of-logrepeat-ind (n width times)
+           (if (zp times)
+               (list n width)
+             (logbitp-of-logrepeat-ind (- (nfix n) (nfix width)) width (1- (nfix times))))))
+
+  (defret logbitp-of-logrepeat
+    (equal (logbitp n reps)
+           (and (< (nfix n) (* (nfix width) (nfix times)))
+                (logbitp (mod (nfix n) (nfix width)) data)))
+    :hints(("Goal" :in-theory (enable bitops::logbitp-of-logapp-split)
+            :induct (logbitp-of-logrepeat-ind n width times))))
+
+  (defthm logrepeat-1
+    (equal (logrepeat 1 width data)
+           (loghead width data))
+    :hints (("goal" :expand ((logrepeat 1 width data)) )))
+
+  
+  (local (defun mod-less-ind (n width)
+           (declare (Xargs :measure (nfix n)))
+           (if (zp n)
+               width
+             (mod-less-ind (- n (* 2 (acl2::pos-fix width))) width))))
+
+  (local (defthm plus-two-minuses
+           (equal (+ (- x) (- x))
+                  (- (* 2 x)))))
+
+  (local (defthm mod-when-less-than-half
+           (implies (and (natp n) (natp w)
+                         (< (mod n (* 2 w)) w))
+                    (equal (mod n (* 2 w))
+                           (mod n w)))
+           :hints (("goal"
+                   :induct (mod-less-ind n w))
+                   (and stable-under-simplificationp
+                        '(:cases ((posp w))))
+                   (and stable-under-simplificationp
+                        '(:cases ((< n (* 2 w))))))))
+
+  (local (defthm mod-when-greater-than-half
+           (implies (and (natp n) (natp w)
+                         (<= w (mod n (* 2 w))))
+                    (equal (mod n (* 2 w))
+                           (+ (mod n w) w)))
+           :hints (("goal"
+                   :induct (mod-less-ind n w))
+                   (and stable-under-simplificationp
+                        '(:cases ((posp w))))
+                   (and stable-under-simplificationp
+                        '(:cases ((< n (* 2 w))))))))
+
+  (defthm logrepeat-2x
+    (implies (natp width)
+             (equal (logrepeat times (* 2 width) (logapp width data data))
+                    (logrepeat (* 2 (nfix times)) width data)))
+    :hints (("goal" :in-theory (disable logrepeat)
+             :do-not-induct t)
+            (bitops::equal-by-logbitp-hammer)))
+
+  (defthm logapp-right-assoc
+    (implies (<= (nfix w2) (nfix w1))
+             (equal (logapp w1 (logapp w2 a b) c)
+                    (logapp w2 a
+                            (logapp (- (nfix w1) (nfix w2)) b c))))
+    :hints ((bitops::logbitp-reasoning)))
+
+  (defthm lognot-of-logrepeat
+    (equal (lognot (logrepeat times width data))
+           (logapp (* (nfix times) (nfix width))
+                   (logrepeat times width (lognot data))
+                   -1))))
+
+
+
+;; e.g. variable 0 initially generates 10
+;; for numvars=4, we need to generate 1010 1010  1010 1010
+;; meaning double it 3 times.  Start with n = 1.
+(define var-repetitions ((n natp) (val natp) (numvars natp))
+  :guard (and (<= n numvars)
+              (unsigned-byte-p (ash 1 n) val))
+  ;; :guard-hints (("goal" :Expand ((ash 1 (+ 1 n)))
+  ;;                :in-theory (enable logcons)))
+  :verify-guards nil
+  ;; :measure (nfix (- (nfix numvars) (nfix n)))
+  :returns (rep-val natp :rule-classes :type-prescription)
+  :enabled t
+  (mbe :logic (logrepeat (ash 1 (- (nfix numvars) (nfix n)))
+                         (ash 1 (nfix n))
+                         (nfix val))
+       :exec (b* ((shift (ash 1 n))
+                  ((when (mbe :logic (zp (- numvars n))
+                              :exec (eql n numvars)))
+                   val))
+               (var-repetitions (+ 1 n)
+                                (logapp shift val val) numvars)))
+  ///
+  (verify-guards var-repetitions
+    :hints(("Goal" :in-theory (e/d* (logcons) (acl2::exponents-add))
+            :expand ((ash 1 (+ (- n) numvars))
+                     (ash 1 (+ 1 n)))))))
+
+  ;; (local (defthmd loghead-less-than-ash-gen-lemma
+  ;;          (implies (natp i)
+  ;;                   (< (loghead m x) (ash 1 (+ i (nfix m)))))
+  ;;          :hints(("Goal" :in-theory (enable* ihsext-inductions
+  ;;                                             ihsext-recursive-redefs)))))
+
+  ;; (local (defthm loghead-less-than-ash-gen
+  ;;          (implies (<= (nfix m) (ifix n))
+  ;;                   (< (loghead m x) (ash 1 n)))
+  ;;          :hints (("goal" :use ((:instance loghead-less-than-ash-gen-lemma
+  ;;                                 (i (- (ifix n) (nfix m)))))))))
+
+  ;; (local (defthm loghead-when-less-than-ash
+  ;;          (implies (and (< (loghead n x) (ash 1 (+ -1 n)))
+  ;;                        (posp n))
+  ;;                   (equal (loghead n x)
+  ;;                          (loghead (1- n) x)))
+  ;;          :hints(("Goal" :in-theory (enable* ihsext-inductions
+  ;;                                             ihsext-recursive-redefs)))))
+
+  ;; (local (defthm logbitp-of-loghead-past-range
+  ;;          (implies (< (nfix n) (nfix m))
+  ;;                   (equal (logbitp n (loghead m x))
+  ;;                          (logbitp n x)))
+  ;;          :hints(("Goal" :in-theory (enable* ihsext-inductions
+  ;;                                            ihsext-recursive-redefs)))))
+
+  ;; (local (defthmd loghead-of-plus-one
+  ;;          (implies (posp n)
+  ;;                   (equal (loghead n env)
+  ;;                          (+ (if (logbitp (1- n) env) (ash 1 (1- n)) 0)
+  ;;                             (loghead (1- n) env))))
+  ;;          :hints(("Goal" :in-theory (enable* loghead** logbitp**
+  ;;                                             ihsext-inductions)
+  ;;                  :induct t)
+  ;;                 (and stable-under-simplificationp
+  ;;                      '(:expand ((ash 1 (+ -1 n)))
+  ;;                        :in-theory (enable logcons))))))
+
+
+
+  ;; (defret var-repetitions-invar
+  ;;   (equal (truth-eval rep-val env numvars)
+  ;;          (truth-eval (nfix val) (loghead n (nfix env)) numvars))
+  ;;   :hints(("Goal" :in-theory (enable truth-eval
+  ;;                                     bitops::logbitp-of-ash-split)
+  ;;           :induct t)
+  ;;          (and stable-under-simplificationp
+  ;;               '(:in-theory (enable loghead-of-plus-one)))))
+
+  ;; (defret var-repetitions-size
+  ;;   (implies (and (<= (nfix n) numvars)
+  ;;                 (natp numvars)
+  ;;                 (unsigned-byte-p (ash 1 (nfix n)) val))
+  ;;            (unsigned-byte-p (ash 1 numvars) rep-val))
+  ;;   :hints (("goal" :induct t
+  ;;            :expand ((ash 1 (+ 1 (nfix n))))
+  ;;            :in-theory (enable logcons))))
+
+
+  ;; (local (defun var-repetitions-masked-size-ind (m n val numvars)
+  ;;          (declare (xargs :measure (nfix (- (nfix numvars) (nfix n)))))
+  ;;          (b* ((n (lnfix n))
+  ;;               (shift (ash 1 n))
+  ;;               (val (mbe :logic (loghead shift (nfix val)) :exec val))
+  ;;               ((when (mbe :logic (zp (- (nfix numvars) n))
+  ;;                           :exec (eql n numvars)))
+  ;;                (list m val)))
+  ;;            (var-repetitions-masked-size-ind
+  ;;             (+ shift m)
+  ;;             (+ 1 n)
+  ;;             (logapp shift val val)
+  ;;             numvars))))
+
+
+  ;; (local (defthm loghead-of-logapp
+  ;;          (implies (<= (nfix w1) (nfix w2))
+  ;;                   (equal (loghead w2 (logapp w1 a b))
+  ;;                          (logapp w1 a (loghead (- (nfix w2) (nfix w1)) b))))
+  ;;          :hints ((bitops::logbitp-reasoning))))
+
+  ;; (local (defthm unsigned-byte-p-implies-width-natp
+  ;;          (implies (unsigned-byte-p n x)
+  ;;                   (natp n))
+  ;;          :hints(("Goal" :in-theory (enable unsigned-byte-p)))
+  ;;          :rule-classes :forward-chaining))
+
+  ;; (local (defthm plus-minus-*-n
+  ;;          (implies (and (syntaxp (quotep n))
+  ;;                        (natp n))
+  ;;                   (equal (+ (- x) (* n x))
+  ;;                          (* (+ -1 n) x)))))
+
+  ;; (defret var-repetitions-negated-masked-size
+  ;;   (implies (and (<= (nfix n) numvars)
+  ;;                 (natp numvars)
+  ;;                 (unsigned-byte-p m (loghead (ash 1 (nfix n)) (lognot (nfix val)))))
+  ;;            (unsigned-byte-p (- (ash 1 numvars) (- (ash 1 (nfix n)) m))
+  ;;                             (loghead (ash 1 numvars) (lognot rep-val))))
+  ;;   :hints (("goal" :induct (var-repetitions-masked-size-ind m n val numvars)
+  ;;            :expand ((ash 1 (+ 1 (nfix n)))
+  ;;                     (var-repetitions n val numvars))
+  ;;            :in-theory (enable logcons))))
+
+  ;; (local (defthm lognot-equal-ash-implies
+  ;;          (implies (and (equal (loghead nn (lognot val))
+  ;;                               (ash val m))
+  ;;                        (natp nn))
+  ;;                   (unsigned-byte-p nn (ash val m)))))
+
+
+  ;; (local (defthmd ash-is-unsigned-byte-p-implies-x-is-unsigned-byte-p
+  ;;          (implies (and (natp m)
+  ;;                        (unsigned-byte-p n (ash x m))
+  ;;                        (natp x))
+  ;;                   (unsigned-byte-p n x))
+  ;;          :hints (("goal" :induct (ash x m)
+  ;;                   :in-theory (enable* ihsext-inductions
+  ;;                                      ihsext-recursive-redefs)))))
+
+  ;; (local (defthm lognot-equal-ash-implies2
+  ;;          (implies (and (equal (loghead nn (lognot val))
+  ;;                               (ash val m))
+  ;;                        (natp m)
+  ;;                        (natp nn)
+  ;;                        (natp val))
+  ;;                   (unsigned-byte-p nn val))
+  ;;          :hints (("goal" :use ((:instance ash-is-unsigned-byte-p-implies-x-is-unsigned-byte-p
+  ;;                                 (x val) (n nn)))))))
+
+  ;; (local (defthm logapp-of-equal-loghead
+  ;;          (implies (and (equal x (loghead n y))
+  ;;                        (syntaxp (not (equal x y))))
+  ;;                   (equal (logapp n x z)
+  ;;                          (logapp n y z)))))
+
+  ;; (local (in-theory (disable loghead-when-less-than-ash))) 
+
+  ;; (local (defthm logapp-of-ash-when-unsigned-byte-p
+  ;;          (implies (And (natp m)
+  ;;                        (equal (loghead nn (ash val m))
+  ;;                               (ash val m)))
+  ;;                   (equal (ash (logapp nn val val2) m)
+  ;;                          (logapp nn (ash val m) (ash val2 m))))
+  ;;          :hints ((bitops::logbitp-reasoning :prune-examples nil))))
+                    
+
+  ;; (local (defthm ash-of-logapp-lemma
+  ;;          (implies (and (equal (loghead nn (lognot val))
+  ;;                               (ash val m))
+  ;;                        (natp m)
+  ;;                        (natp val))
+  ;;                   (equal (ash (logapp nn val val) m)
+  ;;                          (logapp nn (lognot val) (ash val m))))
+  ;;          :hints ((bitops::logbitp-reasoning :prune-examples nil)
+  ;;                  '(:do-not-induct t))))
+
+
+  ;; (local (defthm ash-of-logapp-lemma
+  ;;          (implies (and (equal (loghead m val) 0)
+  ;;                        (< (nfix m) (nfix nn)))
+  ;;                   (equal (logtail m (logapp nn val2 val))
+  ;;                          (logapp nn (logtail m (loghead nn val2)) (logtail m val))))
+  ;;          :hints ((bitops::logbitp-reasoning :prune-examples nil)
+  ;;                  '(:do-not-induct t))
+  ;;          :otf-flg t))
+
+  ;; ;; (defthm tail-equals-head-of-lognot-implies-head-0
+  ;; ;;   (implies (equal (loghead n (lognot val))
+  ;; ;;                   (logtail m val))
+  ;; ;;            (equal (loghead m val) 0))
+  ;; ;;   :hints ((bitops::logbitp-reasoning :prune-examples nil)))
+
+  ;; (local (defthm loghead-of-logapp-when-less
+  ;;          (implies (<= (nfix n) (nfix m))
+  ;;                   (equal (loghead n (logapp m a b))
+  ;;                          (loghead n a)))
+  ;;          :hints ((bitops::logbitp-reasoning))))
+
+  ;; (defret var-repetitions-negated
+  ;;   (implies (and (posp n)
+  ;;                 (<= n numvars)
+  ;;                 (< (nfix m) (ash 1 n))
+  ;;                 (natp numvars)
+  ;;                 (equal (loghead (ash 1 (nfix n)) (lognot (nfix val)))
+  ;;                        (logtail m (nfix val)))
+  ;;                 (equal (loghead m (nfix val)) 0))
+  ;;            (equal (loghead (ash 1 numvars) (lognot rep-val))
+  ;;                   (logtail m rep-val)))
+  ;;   :hints (("goal" :induct t
+  ;;            :expand ((ash 1 (+ 1 n)))
+  ;;            :in-theory (enable logcons)))))
 
 (local (defthm posp-of-ash-1
          (implies (not (negp n))
@@ -247,6 +488,23 @@
               (<= (ash 1 (nfix n)) (loghead (+ 1 (nfix n)) x)))
          :hints(("Goal" :in-theory (enable* ihsext-inductions
                                             ihsext-recursive-redefs)))))
+
+(local
+ (defthmd ash-1-monotonic
+   (implies (and (< a b)
+                 (natp a)
+                 (integerp b))
+            (< (ash 1 a)
+               (ash 1 b)))
+   :hints(("Goal" :in-theory (enable bitops::ash-is-expt-*-x)))
+   :rule-classes ((:rewrite) (:linear))))
+
+(local (defthmd loghead-less-than-ash
+         (implies (not (negp n))
+                  (< (loghead n x) (ash 1 n)))
+         :hints(("Goal" :in-theory (enable* ihsext-inductions
+                                            ihsext-recursive-redefs)))
+         :rule-classes (:rewrite :linear)))
 
 (define var ((n natp) (numvars natp))
   :guard (< n numvars)
@@ -262,12 +520,6 @@
        (rep (ash (logmask w) w)))
     (var-repetitions (+ 1 n) rep numvars))
   ///
-  
-  (local (defthmd loghead-less-than-ash
-           (implies (not (negp n))
-                    (< (loghead n x) (ash 1 n)))
-           :hints(("Goal" :in-theory (enable* ihsext-inductions
-                                              ihsext-recursive-redefs)))))
 
   (local (defthm loghead-less-than-ash-times-2-linear
            (implies (natp n)
@@ -278,30 +530,49 @@
                     :in-theory (enable logcons)))
            :rule-classes :linear))
 
+  (local (defthm product-of-ash
+           (implies (and (natp a) (natp b))
+                    (equal (* (ash 1 a) (ash 1 b))
+                           (ash 1 (+ a b))))
+           :hints(("Goal" :in-theory (enable bitops::ash-is-expt-*-x)))))
+
+  (local (defthm mod-of-ash-1-is-loghead
+           (implies (and (natp n) (integerp x))
+                    (equal (mod x (ash 1 n))
+                           (loghead n x)))
+           :hints(("Goal" :in-theory (enable loghead
+                                             bitops::ash-is-expt-*-x)))))
+
+  (defret logbitp-of-var
+    (implies (< (nfix n) (nfix numvars))
+             (equal (logbitp env var-enc)
+                    (and (< (nfix env) (ash 1 numvars))
+                         (logbitp n (nfix env)))))
+    :hints ((and stable-under-simplificationp
+                 '(:in-theory (enable ;; truth-eval env-lookup
+                                      bitops::logbitp-of-ash-split
+                                      loghead-less-than-ash
+                                      )))
+            (and stable-under-simplificationp
+                 '(:in-theory (enable logbitp-in-terms-of-loghead)))))
+    ;; :hints (("goal" :use eval-of-var
+    ;;          :in-theory (e/d (truth-eval env-lookup)
+    ;;                          (eval-of-var var)))))
+
   (defret eval-of-var
     (implies (< (nfix n) (nfix numvars))
              (equal (truth-eval var-enc env numvars)
                     (env-lookup n env)))
-    :hints ((and stable-under-simplificationp
-                 '(:in-theory (enable truth-eval env-lookup
-                                      bitops::logbitp-of-ash-split)))
-            (and stable-under-simplificationp
-                 '(:in-theory (enable logbitp-in-terms-of-loghead)))))
-
-  (defret logbitp-of-var
-    (implies (and (< (nfix n) (nfix numvars))
-                  (unsigned-byte-p numvars env))
-             (equal (logbitp env var-enc)
-                    (logbitp n env)))
-    :hints (("goal" :use eval-of-var
-             :in-theory (e/d (truth-eval env-lookup)
-                             (eval-of-var var)))))
+    :hints (("goal" :in-theory (e/d (truth-eval env-lookup
+                                                loghead-less-than-ash)
+                                    (var)))))
 
   (defret var-size-basic
     (implies (and (< (nfix n) numvars)
                   (natp numvars))
              (unsigned-byte-p (ash 1 numvars) var-enc))
-    :hints (("goal" :expand ((ash 1 (+ 1 (nfix n))))
+    :hints (("goal" :expand ((ash 1 (+ 1 (nfix n)))
+                             (ash 1 numvars))
              :in-theory (enable logcons))))
 
   (defret var-size
@@ -341,28 +612,103 @@
            (equal (loghead n (lognot (logmask n))) 0)
            :hints ((bitops::logbitp-reasoning))))
 
+  (local (defthm var-negated-masked-lemma
+           (implies (natp n)
+                    (equal (LOGHEAD (* 2 n)
+                                    (LOGAPP n
+                                            -1
+                                            (LOGNOT (LOGMASK n))))
+                           (logmask n)))
+           :hints ((bitops::logbitp-reasoning))))
+
+  (local (defthm plus-minus-times-2
+           (equal (+ n (- (* 2 n)) m)
+                  (+ (- n) m))))
+
+  
+
   (defret var-negated-masked-size
     (implies (and (< (nfix n) numvars)
                   (natp numvars))
              (unsigned-byte-p (- (ash 1 numvars) (ash 1 (nfix n)))
                               (loghead (ash 1 numvars) (lognot var-enc))))
-    :hints (("Goal" :use ((:instance var-repetitions-negated-masked-size
-                           (n (+ 1 (nfix n)))
+    :hints (("Goal" :use ((:instance size-of-logrepeat-by-data-size
+                           (n (+ (ash 1 numvars) (- (ash 1 (nfix n)))))
                            (m (ash 1 (nfix n)))
-                           (val (ash (logmask (ash 1 (nfix n))) (ash 1 (nfix n))))))
-             :expand ((ash 1 (+ 1 (nfix n))))
-             :in-theory (e/d (logcons)
-                             (var-repetitions-negated-masked-size))))))
+                           (times (ash 1 (+ -1 numvars (- (nfix n)))))
+                           (width (ash 1 (+ 1 (nfix n))))
+                           (data (LOGAPP (ASH 1 (NFIX N))
+                                      -1
+                                      (LOGNOT (LOGMASK (ASH 1 (NFIX N)))))))
+                          (:instance var-negated-masked-lemma
+                           (n (ash 1 (nfix n)))))
+             :expand ((ash 1 (+ 1 (nfix n)))
+                      (ash 1 numvars))
+             :in-theory (e/d (logcons
+                              ash-1-monotonic)
+                             (size-of-logrepeat-by-data-size
+                              var-negated-masked-lemma))))
+    ;; :hints (("Goal" :use ((:instance var-repetitions-negated-masked-size
+    ;;                        (n (+ 1 (nfix n)))
+    ;;                        (m (ash 1 (nfix n)))
+    ;;                        (val (ash (logmask (ash 1 (nfix n))) (ash 1 (nfix n))))))
+    ;;          :expand ((ash 1 (+ 1 (nfix n))))
+    ;;          :in-theory (e/d (logcons)
+    ;;                          (var-repetitions-negated-masked-size))))
+    )
 
+  (local (defthm loghead-of-plus-last-bit
+           (implies (and (natp n) (integerp x))
+                    (equal (loghead (+ 1 n) (+ x (ash 1 n)))
+                           (if (< (loghead (+ 1 n) x) (ash 1 n))
+                               (+ (loghead (+ 1 n) x) (ash 1 n))
+                             (- (loghead (+ 1 n) x) (ash 1 n)))))
+           :hints (("goal" :induct (loghead n x)
+                    :in-theory (enable* ihsext-inductions
+                                       ihsext-recursive-redefs
+                                       logcons)))))
+
+  (local (defun less-when-loghead-less-ind (w n num)
+           (if (zp n)
+               (list w num)
+             (less-when-loghead-less-ind (logcdr w) (1- n) (1- num)))))
+
+  (local (defthm not-even-when-loghead-0
+           (implies (and (equal (logcar x) 1)
+                         (integerp y))
+                    (not (equal (* 2 y) x)))))
+
+  (local (defthm less-when-loghead-less
+           (implies (and (integerp w)
+                         (natp num) (natp n)
+                         (< n num)
+                         (< w (ash 1 num))
+                         (< (loghead (+ 1 n) w) (ash 1 n)))
+                    (< (+ w (ash 1 n)) (ash 1 num)))
+           :hints (("goal" :induct (less-when-loghead-less-ind w n num)
+                    :expand ((loghead (+ 1 n) w)
+                             (loghead 1 w)
+                             (ash 1 n)
+                             (ash 1 num))
+                    :in-theory (enable logcons)))))
+
+  (defret var-negated
+    (implies (and (< (nfix n) numvars)
+                  (natp numvars))
+             (equal (loghead (ash 1 numvars) (lognot var-enc))
+                    (logtail (ash 1 (nfix n)) var-enc)))
+    :hints ((bitops::logbitp-reasoning))))
+
+(local (defthmd loghead-less-than-ash-nfix
+         (< (loghead n x) (ash 1 (nfix n)))
+         :hints(("Goal" :in-theory (enable* ihsext-inductions
+                                            ihsext-recursive-redefs)))))
 
 (define truth-norm ((truth integerp) (numvars natp))
   :returns (norm-truth)
   (loghead (ash 1 (lnfix numvars)) truth)
   ///
-  (local (defthm loghead-less-than-ash-nfix
-           (< (loghead n x) (ash 1 (nfix n)))
-           :hints(("Goal" :in-theory (enable* ihsext-inductions
-                                              ihsext-recursive-redefs)))))
+  (local (in-theory (enable loghead-less-than-ash-nfix)))
 
   (local (defthm logbitp-of-loghead-past-range
            (implies (< (nfix n) (nfix m))
@@ -469,6 +815,12 @@
                            (not (logbitp n x))))
            :hints(("Goal" :in-theory (enable* ihsext-inductions
                                               ihsext-recursive-redefs)))))
+
+  (local (defthm <-ash-by-unsigned-byte-p
+           (implies (unsigned-byte-p n x)
+                    (< x (ash 1 n)))
+           :hints(("Goal" :in-theory (enable unsigned-byte-p
+                                             bitops::ash-is-expt-*-x)))))
 
   (defret positive-cofactor-correct
     (implies (< (nfix n) (nfix numvars))
@@ -670,7 +1022,8 @@
              (unsigned-byte-p (ash 1 numvars) cofactor))
     :hints (("goal" :use ((:instance size-of-logand-by-size-of-loghead
                            (a (loghead (ash 1 numvars) truth)) (b (lognot (var n numvars)))
-                           (m (ash 1 numvars)) (n (- (ash 1 numvars) (ash 1 (nfix n)))))))))
+                           (m (ash 1 numvars)) (n (- (ash 1 numvars) (ash 1 (nfix n))))))
+             :in-theory (enable ash-1-monotonic))))
 
   (defret negative-cofactor-size
     (implies (and (natp m)
@@ -723,32 +1076,625 @@
              :cases ((env-lookup n env))))))
          
   
+;; (define swap-vars ((n natp) (m natp) (truth integerp) (numvars natp))
+;;   :guard (and (< n numvars) (< m numvars))
+;;   :returns (swapped-truth integerp :rule-classes :type-prescription)
+;;   (b* ((xn1 (positive-cofactor n truth numvars))
+;;        (xn0 (negative-cofactor n truth numvars))
+;;        (xn1m1 (positive-cofactor m xn1 numvars))
+;;        (xn1m0 (negative-cofactor m xn1 numvars))
+;;        (xn0m1 (positive-cofactor m xn0 numvars))
+;;        (xn0m0 (negative-cofactor m xn0 numvars))
+;;        (mvar (var m numvars))
+;;        (nvar (var n numvars))
+;;        (~mvar (lognot mvar))
+;;        (~nvar (lognot nvar))
+;;        ;; want (if n (if m xn1m1 xn0m1) (if m xn1m0 xn0m0))
+;;        (n1case (logior (logand mvar xn1m1)
+;;                        (logand ~mvar xn0m1)))
+;;        (n0case (logior (logand mvar xn1m0)
+;;                        (logand ~mvar xn0m0))))
+;;     (logior (logand nvar n1case)
+;;             (logand ~nvar n0case)))
+;;   ///
+;;   (defret eval-of-swap-vars
+;;     (implies (and (< (nfix n) (nfix numvars))
+;;                   (< (nfix m) (nfix numvars)))
+;;              (equal (truth-eval swapped-truth env numvars)
+;;                     (truth-eval truth
+;;                                 (env-update n (env-lookup m env)
+;;                                             (env-update m (env-lookup n env) env))
+;;                                 numvars)))))
+
+
+(defsection logbitp-loghead-of-add-theory
+  (local (defun logbitp-of-plus-ind (n c a b)
+           (if (zp n)
+               (list a b c)
+             (logbitp-of-plus-ind
+              (1- n) (b-ior (b-and (logcar a) (logcar b))
+                            (b-ior (b-and c (logcar a))
+                                   (b-and c (logcar b))))
+              (logcdr a) (logcdr b)))))
+
+  (local (defthm logbitp-of-plus-lemma
+           (implies (and (integerp a) (integerp b) (bitp c))
+                    (Equal (logbitp n (+ c a b))
+                           (equal 1 (b-xor (logbit n a)
+                                           (b-xor (logbit n b)
+                                                  (bool->bit
+                                                   (<= (ash 1 (nfix n))
+                                                       (+ c (loghead n a)
+                                                          (loghead n b)))))))))
+           :hints (("goal" :induct (logbitp-of-plus-ind n c a b)
+                    :in-theory (e/d* (logcons
+                                      bool->bit b-and bitp)
+                                     ( ;; loghead-by-bounds
+                                      acl2::loghead-identity
+                                      bitops::logbitp-when-bitmaskp))
+                    :expand ((:free (x) (logbitp n x))
+                             (:free (x) (loghead n x))
+                             (:free (x) (logbitp 0 x))
+                             (ash 1 (nfix n))
+                             (ash 1 n))))))
+
+  (defthmd logbitp-of-plus
+    (implies (and (integerp a) (integerp b))
+             (Equal (logbitp n (+ a b))
+                    (equal 1 (b-xor (logbit n a)
+                                    (b-xor (logbit n b)
+                                           (bool->bit
+                                            (<= (ash 1 (nfix n))
+                                                (+ (loghead n a)
+                                                   (loghead n b)))))))))
+    :hints (("Goal" :use ((:instance logbitp-of-plus-lemma
+                           (c 0))))))
+
+
+  (local (defthm loghead-of-plus-lemma
+           (implies (and (integerp a) (integerp b) (bitp c))
+                    (Equal (loghead n (+ c a b))
+                           (let ((sum (+ c (loghead n a) (loghead n b))))
+                             (if (<= (ash 1 (nfix n)) sum)
+                                 (- sum (ash 1 (nfix n)))
+                               sum))))
+           :hints (("goal" :induct (logbitp-of-plus-ind n c a b)
+                    :in-theory (e/d* (
+                                     logcons
+                                     bool->bit b-and bitp)
+                                     ( ;; loghead-by-bounds
+                                      acl2::loghead-identity))
+                    :expand ((:free (x) (loghead n x))
+                             (ash 1 (nfix n))
+                             (ash 1 n))))))
+
+  (defthmd loghead-of-plus
+    (implies (and (integerp a) (integerp b))
+             (Equal (loghead n (+ a b))
+                    (let ((sum (+ (loghead n a) (loghead n b))))
+                      (if (<= (ash 1 (nfix n)) sum)
+                          (- sum (ash 1 (nfix n)))
+                        sum))))
+    :hints (("Goal" :use ((:instance loghead-of-plus-lemma
+                           (c 0)))))))
+
+
+;; BOZO consider moving these to shareable books
+(local
+ (defsection logbitp-of-plus-nonoverlap-theory
+
+   (local (defun logbitp-ash-ind (n m x)
+            (if (zp n)
+                (list m x)
+              (logbitp-ash-ind (1- n) (1- m) (logcdr x)))))
+
+   (defthm logbitp-of-plus-ash-unset
+     (implies (and (integerp x)
+                   (natp m)
+                   (not (logbitp (double-rewrite m) x)))
+              (equal (logbitp n (+ x (ash 1 m)))
+                     (or (equal (nfix n) m) (logbitp n x))))
+     :hints (("goal" :induct (logbitp-ash-ind n m x)
+              :in-theory (enable* ihsext-recursive-redefs))))
+
+   (local (defthm logcdr-minus-logcons-0
+            (equal (logcdr (- (logcons 0 x)))
+                   (- (ifix x)))
+            :hints(("Goal" :in-theory (enable bitops::minus-to-lognot)))))
+
+   (defthm logbitp-of-plus-ash-unset-2
+     (implies (and (integerp x)
+                   (natp m)
+                   (not (logbitp (double-rewrite m) x)))
+              (equal (logbitp n (+ (ash 1 m) x))
+                     (or (equal (nfix n) m) (logbitp n x)))))
+
+   (defthm logbitp-of-plus-ash-unset-3
+     (implies (and (integerp x) (integerp y)
+                   (natp m)
+                   (not (logbitp (double-rewrite m) (+ x y))))
+              (equal (logbitp n (+ x (ash 1 m) y))
+                     (or (equal (nfix n) m) (logbitp n (+ x y)))))
+     :hints (("Goal" :use ((:instance logbitp-of-plus-ash-unset-2
+                            (x (+ x y)))))))
+
+   (defthm logbitp-of-minus-ash-set
+     (implies (and (integerp x)
+                   (natp m)
+                   (logbitp (double-rewrite m) x))
+              (equal (logbitp n (+ x (- (ash 1 m))))
+                     (and (not (equal (nfix n) m)) (logbitp n x))))
+     :hints (("goal" :induct (logbitp-ash-ind n m x)
+              :in-theory (enable* ihsext-recursive-redefs)
+              :expand ((:free (x) (logbitp n x))
+                       (:free (x) (logbitp m x))))))
+
+
+   (defthm logbitp-of-minus-ash-set-2
+     (implies (and (integerp x)
+                   (natp m)
+                   (logbitp (double-rewrite m) x))
+              (equal (logbitp n (+ (- (ash 1 m)) x))
+                     (and (not (equal (nfix n) m)) (logbitp n x)))))
+
+   (defthm logbitp-of-minus-ash-set-3
+     (implies (and (integerp x) (integerp y)
+                   (natp m)
+                   (logbitp (double-rewrite m) (+ x y)))
+              (equal (logbitp n (+ x (- (ash 1 m)) y))
+                     (and (not (equal (nfix n) m)) (logbitp n (+ x y)))))
+     :hints (("Goal" :use ((:instance logbitp-of-minus-ash-set-2
+                            (x (+ x y)))))))
+
+   (defthm loghead-of-plus-ash-unset
+     (implies (and (integerp x)
+                   (natp m)
+                   (not (logbitp (double-rewrite m) x)))
+              (equal (loghead n (+ x (ash 1 m)))
+                     (+ (if (<= (nfix n) m) 0 (ash 1 m))
+                        (loghead n x))))
+     :hints (("goal" :induct (logbitp-ash-ind n m x)
+              :in-theory (enable* ihsext-recursive-redefs logcons))))
+
+   
+   (defthm loghead-of-plus-ash-unset-2
+     (implies (and (integerp x)
+                   (natp m)
+                   (not (logbitp (double-rewrite m) x)))
+              (equal (loghead n (+ (ash 1 m) x))
+                     (+ (if (<= (nfix n) m) 0 (ash 1 m))
+                        (loghead n x)))))
+
+   (defthm loghead-of-plus-ash-unset-3
+     (implies (and (integerp x) (integerp y)
+                   (natp m)
+                   (not (logbitp (double-rewrite m) (+ x y))))
+              (equal (loghead n (+ x (ash 1 m) y))
+                     (+ (if (<= (nfix n) m) 0 (ash 1 m))
+                        (loghead n (+ x y)))))
+     :hints (("Goal" :use ((:instance loghead-of-plus-ash-unset-2
+                            (x (+ x y)))))))
+
+
+   (local (defthm logcdr-minus-2x
+            (implies (integerp x)
+                     (equal (logcdr (- (* 2 x)))
+                            (- x)))
+            :hints(("Goal" :use ((:instance bitops::logcdr-of-logcons
+                                  (x (- x)) (b 0)))
+                    :in-theory (e/d (logcons) (bitops::logcdr-of-logcons))))))
+   
+   (defthm loghead-of-minus-ash-set
+     (implies (and (integerp x)
+                   (natp m)
+                   (logbitp (double-rewrite m) x))
+              (equal (loghead n (+ x (- (ash 1 m))))
+                     (+ (if (<= (nfix n) m) 0 (- (ash 1 m)))
+                        (loghead n x))))
+     :hints (("goal" :induct (logbitp-ash-ind n m x)
+              :in-theory (enable* ihsext-recursive-redefs logcons)
+              :expand ((:free (x) (loghead n x))
+                       (:free (x) (loghead m x))))))
+
+
+   (defthm loghead-of-minus-ash-set-2
+     (implies (and (integerp x)
+                   (natp m)
+                   (logbitp (double-rewrite m) x))
+              (equal (loghead n (+ (- (ash 1 m)) x))
+                     (+ (if (<= (nfix n) m) 0 (- (ash 1 m)))
+                        (loghead n x)))))
+
+   (defthm loghead-of-minus-ash-set-3
+     (implies (and (integerp x) (integerp y)
+                   (natp m)
+                   (logbitp (double-rewrite m) (+ x y)))
+              (equal (loghead n (+ x (- (ash 1 m)) y))
+                     (+ (if (<= (nfix n) m) 0 (- (ash 1 m)))
+                        (loghead n (+ x y)))))
+     :hints (("Goal" :use ((:instance loghead-of-minus-ash-set-2
+                            (x (+ x y)))))))
+
+   ))
+
+(local
+ (defsection logbitp-of-plus-ash-same-theory
+
+   (defthm logbitp-of-plus-ash
+     (implies (and (integerp x))
+              (equal (logbitp m (+ x (ash 1 (nfix m))))
+                     (not (logbitp m x))))
+     :hints(("Goal" :in-theory (enable* ihsext-inductions
+                                        ihsext-recursive-redefs))))
+
+   (defthm logbitp-of-plus-ash-2
+     (implies (and (equal mm (nfix m))
+                   (integerp x) (integerp y))
+              (equal (logbitp m (+ x (ash 1 mm) y))
+                     (not (logbitp m (+ x y)))))
+     :hints (("Goal" :use ((:instance logbitp-of-plus-ash
+                            (x (+ x y))))
+              :in-theory (disable logbitp-of-plus-ash))))
+
+   (defthm logbitp-of-plus-ash-3
+     (implies (and (equal mm (nfix m))
+                   (integerp x) (integerp y))
+              (equal (logbitp m (+ x y (ash 1 mm)))
+                     (not (logbitp m (+ x y)))))
+     :hints (("Goal" :use ((:instance logbitp-of-plus-ash
+                            (x (+ x y))))
+              :in-theory (disable logbitp-of-plus-ash))))
+
+   (defthm logbitp-of-minus-ash
+     (implies (and (natp m) (integerp x))
+              (equal (logbitp m (+ x (- (ash 1 m))))
+                     (not (logbitp m x))))
+     :hints (("Goal" :use ((:instance logbitp-of-plus-ash
+                            (x (+ x (- (ash 1 m))))))
+              :in-theory (disable logbitp-of-plus-ash))))
+
+   (defthm logbitp-of-minus-ash-2
+     (implies (and (natp m) (integerp x))
+              (equal (logbitp m (+ (- (ash 1 m)) x))
+                     (not (logbitp m x))))
+     :hints (("Goal" :use ((:instance logbitp-of-plus-ash
+                            (x (+ x (- (ash 1 m))))))
+              :in-theory (disable logbitp-of-plus-ash))))
+
+   (defthm logbitp-of-minus-ash-3
+     (implies (and (equal mm (nfix m))
+                   (integerp x) (integerp y))
+              (equal (logbitp m (+ x (- (ash 1 mm)) y))
+                     (not (logbitp m (+ x y)))))
+     :hints (("Goal" :use ((:instance logbitp-of-minus-ash
+                            (x (+ x y)) (m mm)))
+              :in-theory (disable logbitp-of-minus-ash))))
+
+   (defthmd logbitp-when-less-than-ash
+     (implies (and (natp n) (< n (ash 1 m))
+                   (natp m))
+              (not (logbitp m n)))
+     :hints(("Goal" :in-theory (enable* ihsext-inductions
+                                        ihsext-recursive-redefs))))))
+
+(defsection complements-related-by-shift
+
+
+  (local (defun loghead-of-plus-ash-ind (m n x)
+           (if (zp m)
+               (list x n)
+             (loghead-of-plus-ash-ind (1- m) (1- (nfix n)) (logcdr x)))))
+
+  (local (defthm logbitp-of-plus-ash-greater
+           (implies (and (< (nfix m) n)
+                         (natp n)
+                         (integerp x))
+                    (equal (logbitp m (+ x (ash 1 n)))
+                           (logbitp m x)))
+           :hints(("Goal" :induct (loghead-of-plus-ash-ind m n x)
+                   :in-theory (enable* ihsext-recursive-redefs)))))
+
+  (local (defthm logbitp-of-minus-ash-greater
+           (implies (and (< (nfix m) n)
+                         (natp n)
+                         (integerp x))
+                    (equal (logbitp m (+ x (- (ash 1 n))))
+                           (logbitp m x)))
+           :hints(("Goal" :use ((:instance logbitp-of-plus-ash-greater
+                                 (x (+ x (- (ash 1 n))))))
+                   :in-theory (disable logbitp-of-plus-ash-greater)))))
+
+  (local (defthm logbitp-of-plus-lesser-when-not-logbitp
+           (implies (and (< (nfix m) n)
+                         (natp n)
+                         (integerp x)
+                         (not (logbitp (double-rewrite m) x)))
+                    (equal (logbitp n (+ x (ash 1 m)))
+                           (logbitp n x)))
+           :hints (("goal" :induct (loghead-of-plus-ash-ind m n x)
+                    :in-theory (enable* ihsext-recursive-redefs)
+                    :expand ((:free (x) (logbitp n x)))))))
+
+  (local (in-theory (enable ash-1-monotonic)))
+
+  (local (defthm loghead-by-bounds
+           (implies (and (<= (ash 1 num) b)
+                         (< b (* 2 (ash 1 num)))
+                         (natp num)
+                         (integerp b))
+                    (equal (loghead num b) (- b (ash 1 num))))
+           :hints(("Goal" :in-theory (enable loghead
+                                             bitops::ash-is-expt-*-x)))))
+
+  
+
+  (local (defthm logbitp-when-bounded-lemma
+           (implies (and (< b (+ (ash 1 n) (- (ash 1 m))))
+                         (natp b) (natp n) (natp m)
+                         (not (logbitp (double-rewrite m) b)))
+                    (not (logbitp n b)))
+           :hints (("Goal" :induct (loghead-of-plus-ash-ind m n b)
+                    :in-theory (enable* ihsext-recursive-redefs
+                                        logcons
+                                        logbitp-when-less-than-ash)))))
+
+  (local (defthm logbitp-when-bounded-lemma2
+           (implies (and (< (+ b (- (ash 1 n)) (ash 1 m))
+                            (ash 1 num))
+                         (natp b) (natp n) (natp m) (< m n)
+                         (natp num) (< n num)
+                         (<= (ash 1 num) b)
+                         (not (logbitp (double-rewrite m) b)))
+                    (not (logbitp n b)))
+           :hints (("goal" :use ((:instance bitops::logbitp-of-loghead-in-bounds
+                                  (pos m) (i b) (size num))
+                                 (:instance bitops::logbitp-of-loghead-in-bounds
+                                  (pos n) (i b) (size num))
+                                 (:instance logbitp-when-bounded-lemma
+                                  (b (loghead num b))))
+                    :in-theory (e/d (ash-1-monotonic)
+                                    (bitops::logbitp-of-loghead-in-bounds
+                                     ;; logbitp-of-minus-ash-greater
+                                     ))))))
+
+  (defthmd complements-related-by-shift
+    (implies (and (< (nfix n) numvars)
+                  (natp numvars)
+                  (< (nfix m) (nfix n)))
+             (equal (logand (var n numvars) (lognot (var m numvars)))
+                    (ash (logand (var m numvars) (lognot (var n numvars)))
+                         (- (ash 1 (nfix n)) (ash 1 (nfix m))))))
+    :hints ((bitops::logbitp-reasoning)
+            (and stable-under-simplificationp
+                 '(:cases ((< bitops::wbit0 (- (ash 1 n) (ash 1 (nfix m))))))))
+    :otf-flg t)
+
+  
+  (local (defthm ash-of-logand
+           (equal (ash (logand a b) sh)
+                  (logand (ash a sh) (ash b sh)))
+           :hints(("Goal" :in-theory (enable* ihsext-inductions
+                                              ihsext-recursive-redefs)))))
+
+
+  (defthm complements-related-by-shift-unshift
+    (implies (and (< (nfix n) numvars)
+                  (natp numvars)
+                  (equal mm (nfix m))
+                  (< (nfix m) (nfix n)))
+             (equal (logand (ash (var m numvars) (+ (ash 1 n) (- (ash 1 mm))))
+                            (ash (lognot (var n numvars)) (+ (ash 1 n) (- (ash 1 mm)))))
+                    (logand (var n numvars) (lognot (var m numvars)))))
+    :hints (("goal" :use ((:instance complements-related-by-shift))
+             :in-theory (disable complements-related-by-shift)))
+    :otf-flg t)
+
+  (defthm complements-related-by-shift-unshift2
+    (implies (and (< (nfix n) numvars)
+                  (natp numvars)
+                  (equal mm (nfix m))
+                  (< (nfix m) (nfix n)))
+             (equal (logand (ash (var m numvars) (+ (- (ash 1 mm)) (ash 1 n)))
+                            (ash (lognot (var n numvars)) (+ (- (ash 1 mm)) (ash 1 n))))
+                    (logand (var n numvars) (lognot (var m numvars)))))
+    :hints (("goal" :use ((:instance complements-related-by-shift))
+             :in-theory (disable complements-related-by-shift)))
+    :otf-flg t)
+
+  (defthm complements-related-by-shift-unshift3
+    (implies (and (< (nfix n) numvars)
+                  (natp numvars)
+                  (equal mm (nfix m))
+                  (< (nfix m) (nfix n)))
+             (equal (logand (ash (var m numvars) (+ (ash 1 n) (- (ash 1 mm))))
+                            (ash (lognot (var n numvars)) (+ (ash 1 n) (- (ash 1 mm))))
+                            z)
+                    (logand (var n numvars) (lognot (var m numvars))
+                            z)))
+    :hints (("goal" :use ((:instance complements-related-by-shift))
+             :in-theory (disable complements-related-by-shift)))
+    :otf-flg t)
+
+  (defthm complements-related-by-shift-untail
+    (implies (and (< (nfix n) numvars)
+                  (natp numvars)
+                  (< (nfix m) (nfix n)))
+             (equal (logand (logtail (+ (ash 1 n) (- (ash 1 (nfix m)))) (var n numvars))
+                            (lognot (logtail (+ (ash 1 n) (- (ash 1 (nfix m)))) (var m numvars))))
+                    (logand (var m numvars) (lognot (var n numvars)))))
+    :hints (("goal" :use ((:instance ash-of-logand
+                           (a (var n numvars)) (b (lognot (var m numvars)))
+                           (sh (- (+ (ash 1 n) (- (ash 1 (nfix m))))))))
+             :in-theory (e/d (complements-related-by-shift))))
+    :otf-flg t)
+
+  (defthm complements-related-by-shift-untail3
+    (implies (and (< (nfix n) numvars)
+                  (natp numvars)
+                  (< (nfix m) (nfix n)))
+             (equal (logand (logtail (+ (ash 1 n) (- (ash 1 (nfix m)))) (var n numvars))
+                            (lognot (logtail (+ (ash 1 n) (- (ash 1 (nfix m)))) (var m numvars)))
+                            z)
+                    (logand (var m numvars) (lognot (var n numvars)) z)))
+    :hints (("goal" :use ((:instance complements-related-by-shift-untail))
+             :in-theory (disable complements-related-by-shift-untail)))
+    :otf-flg t))
+
+
+
 (define swap-vars ((n natp) (m natp) (truth integerp) (numvars natp))
-  :guard (and (< n numvars) (< m numvars))
+  :guard (and (< n numvars) (< m n))
   :returns (swapped-truth integerp :rule-classes :type-prescription)
-  (b* ((xn1 (positive-cofactor n truth numvars))
-       (xn0 (negative-cofactor n truth numvars))
-       (xn1m1 (positive-cofactor m xn1 numvars))
-       (xn1m0 (negative-cofactor m xn1 numvars))
-       (xn0m1 (positive-cofactor m xn0 numvars))
-       (xn0m0 (negative-cofactor m xn0 numvars))
-       (mvar (var m numvars))
-       (nvar (var n numvars))
-       (~mvar (lognot mvar))
-       (~nvar (lognot nvar))
-       ;; want (if n (if m xn1m1 xn0m1) (if m xn1m0 xn0m0))
-       (n1case (logior (logand mvar xn1m1)
-                       (logand ~mvar xn0m1)))
-       (n0case (logior (logand mvar xn1m0)
-                       (logand ~mvar xn0m0))))
-    (logior (logand nvar n1case)
-            (logand ~nvar n0case)))
+  (b* ((truth (loghead (ash 1 (lnfix numvars)) truth))
+       (varn (var n numvars))
+       (varm (var m numvars))
+       (same (logeqv varn varm))
+       (n&~m (logand varn (lognot varm)))
+       (m&~n (logand varm (lognot varn)))
+       (shift (- (ash 1 (lnfix n)) (ash 1 (lnfix m)))))
+    (logior (logand same truth)
+            (ash (logand n&~m truth) (- shift))
+            (ash (logand m&~n truth) shift)))
   ///
+  (local (defthm loghead-over-install-bit
+           (implies (< (nfix n) (nfix w))
+                    (equal (loghead w (install-bit n b x))
+                           (install-bit n b (loghead w x))))
+           :hints ((bitops::logbitp-reasoning)
+                   (and stable-under-simplificationp
+                        '(:in-theory (enable bitops::logbitp-of-install-bit-split
+                                             bitops::logbitp-of-loghead-split))))))
+
+  (local (defthmd logcdr-when-not-integerp
+           (implies (not (integerp x))
+                    (equal (logcdr x) 0))
+           :hints(("Goal" :in-theory (enable logcdr)))))
+  (local (defthmd logcar-when-not-integerp
+           (implies (not (integerp x))
+                    (equal (logcar x) 0))
+           :hints(("Goal" :in-theory (enable logcar)))))
+
+  (local (defthmd install-bit-1-when-not-set
+           (implies (not (logbitp n x))
+                    (equal (install-bit n 1 x)
+                           (+ (Ash 1 (nfix n)) (ifix x))))
+           :hints(("Goal" :in-theory (enable* ihsext-inductions
+                                              ihsext-recursive-redefs
+                                              install-bit**
+                                              logcons
+                                              logcar-when-not-integerp
+                                              logcdr-when-not-integerp)))))
+
+  
+
+  (local (defthmd install-bit-0-when-set
+           (implies (logbitp n x)
+                    (equal (install-bit n 0 x)
+                           (+ (- (Ash 1 (nfix n))) (ifix x))))
+           :hints(("Goal" :in-theory (enable* ihsext-inductions
+                                              ihsext-recursive-redefs
+                                              install-bit**
+                                              logcons
+                                              logcar-when-not-integerp
+                                              logcdr-when-not-integerp)))))
+
+
+
+  (local (defthm loghead->=-ash-when-logbitp
+           (implies (and (logbitp n env)
+                         (natp n) (natp numvars)
+                         (< n numvars))
+                    (<= (ash 1 n) (loghead numvars env)))
+           :hints (("goal" :use ((:instance bitops::logbitp-of-loghead-in-bounds
+                                  (pos n) (i env) (size numvars)))
+                    :in-theory (e/d (logbitp-when-less-than-ash)
+                                    (bitops::logbitp-of-loghead-in-bounds))))
+           :rule-classes :linear)) 
+
+
+  (local (defthmd swap-bits-is-add
+           (implies (and (equal b1 (bool->bit (logbitp m x)))
+                         (equal b2 (bool->bit (logbitp n x))))
+                    (equal (install-bit n b1 (install-bit m b2 x))
+                           (if (xor (logbitp n x)
+                                    (logbitp m x))
+                               (if (logbitp n x)
+                                   (+ (- (ash 1 (nfix n))) (ash 1 (nfix m)) (ifix x))
+                                 (+ (ash 1 (nfix n)) (- (ash 1 (nfix m))) (ifix x)))
+                             (ifix x))))
+           :hints(("goal" :use ((:instance install-bit-0-when-set
+                                 (x (install-bit m (bool->bit (logbitp n x))
+                                                     x)))
+                                (:instance install-bit-1-when-not-set
+                                 (x (install-bit m (bool->bit (logbitp n x))
+                                                     x))))
+                   :in-theory (enable bitops::logbitp-of-install-bit-split))
+                  (and stable-under-simplificationp
+                       '(:use ((:instance install-bit-0-when-set
+                                (n m))
+                               (:instance install-bit-1-when-not-set
+                                (n m))))))))
+
+  (local (defthm ash-of-logand
+           (equal (ash (logand a b) sh)
+                  (logand (ash a sh) (ash b sh)))
+           :hints(("Goal" :in-theory (enable* ihsext-inductions
+                                              ihsext-recursive-redefs)))))
+  
+  (local (in-theory (disable BITOPS::INSTALL-BIT-OF-INSTALL-BIT-DIFF
+                             BITOPS::LOGTAIL-OF-LOGHEAD)))
+
+  (local (defthmd truth-eval-with-loghead
+           (equal (truth-eval truth env numvars)
+                  (logbitp (loghead (nfix numvars) (nfix env))
+                           (loghead (ash 1 (nfix numvars)) truth)))
+           :hints (("Goal" :use truth-eval-of-truth-norm
+                    :in-theory (e/d (truth-eval truth-norm)
+                                    (truth-eval-of-truth-norm))))
+           :rule-classes ((:definition :install-body t))))
+
   (defret eval-of-swap-vars
     (implies (and (< (nfix n) (nfix numvars))
-                  (< (nfix m) (nfix numvars)))
+                  (< (nfix m) (nfix n)))
              (equal (truth-eval swapped-truth env numvars)
                     (truth-eval truth
                                 (env-update n (env-lookup m env)
                                             (env-update m (env-lookup n env) env))
-                                numvars)))))
+                                numvars)))
+    :hints(("Goal" :in-theory (e/d (ash-1-monotonic)
+                                   (truth-eval-of-logand
+                                    truth-eval-of-logior
+                                    truth-eval-of-lognot
+                                    truth-eval-of-logxor)))
+           (and stable-under-simplificationp
+                '(:in-theory (enable env-update env-lookup
+                                     loghead-less-than-ash
+                                     ash-1-monotonic)
+                  :expand ((:with truth-eval (:free (x) (truth-eval x env numvars)))
+                           (:with truth-eval-with-loghead (:free (env) (truth-eval truth env numvars))))))
+           (and stable-under-simplificationp
+                '(:in-theory (enable swap-bits-is-add
+                                     bitops::logbitp-of-loghead-split
+                                     loghead-less-than-ash
+                                     ash-1-monotonic)))
+           (and stable-under-simplificationp
+                '(:in-theory (enable loghead-less-than-ash)
+                  :use ((:instance ash-1-monotonic
+                         (a (nfix m)) (b n))))))
+    :otf-flg t)
+
+  (local (defret size-of-swap-vars-lemma
+           (implies (and (< (nfix n) (nfix numvars))
+                         (< (nfix m) (nfix n)))
+                    (unsigned-byte-p (ash 1 numvars) swapped-truth))
+           :hints(("Goal" :in-theory (enable ash-1-monotonic)))))
+
+  (defret size-of-swap-vars
+    (implies (and (< (nfix n) (nfix numvars))
+                  (< (nfix m) (nfix n))
+                  (natp size)
+                  (<= (ash 1 numvars) size))
+             (unsigned-byte-p size swapped-truth))
+    :hints (("goal" :use size-of-swap-vars-lemma
+             :in-theory (disable size-of-swap-vars-lemma swap-vars)))))
+
