books/centaur/truth/sizes.lisp
@@ -32,6 +32,12 @@
 (in-package "TRUTH")
 
 (include-book "truth")
+(local (include-book "centaur/bitops/ihsext-basics" :dir :system))
+(local (include-book "centaur/bitops/signed-byte-p" :dir :system))
+(local (include-book "centaur/bitops/ash-bounds" :dir :system))
+(local (include-book "arithmetic/top-with-meta" :dir :system))
+(local (include-book "std/basic/arith-equivs" :dir :system))
+(local (in-theory (disable unsigned-byte-p signed-byte-p)))
 
 (define var-alist ((n natp) (numvars natp))
   :guard (<= n numvars)
@@ -53,16 +59,188 @@
   `(case ,n
      . ,(var-cases-fn numvars numvars)))
 
+(defun swap-adjacent-case (m numvars)
+  `(logior (the (unsigned-byte ,(ash 1 numvars))
+                (logand ,(loghead (ash 1 numvars)
+                                  (logeqv (var m numvars)
+                                          (var (+ 1 m) numvars)))
+                        (the (unsigned-byte ,(ash 1 numvars)) truth)))
+           (the (unsigned-byte ,(ash 1 numvars))
+                (ash (the (unsigned-byte ,(ash 1 numvars))
+                          (logand ,(logand (var (+ 1 m) numvars)
+                                           (lognot (var m numvars)))
+                                  (the (unsigned-byte ,(ash 1 numvars)) truth)))
+                     ,(- (ash 1 m))))
+           (the (unsigned-byte ,(ash 1 numvars))
+                (ash (the (unsigned-byte ,(ash 1 numvars))
+                          (logand ,(logand (var m numvars)
+                                           (lognot (var (+ 1 m) numvars)))
+                                  (the (unsigned-byte ,(ash 1 numvars)) truth)))
+                     ,(ash 1 m)))))
+
+(defun swap-adjacent-cases-fn (m numvars)
+  (if (zp m)
+      nil
+    (cons (list (if (eql m 1) 'otherwise (1- m))
+                (swap-adjacent-case (1- m) numvars))
+          (swap-adjacent-cases-fn (1- m) numvars))))
+
+(defmacro swap-adjacent-cases (numvars)
+  `(case m
+     . ,(swap-adjacent-cases-fn (1- numvars) numvars)))
+
+
+(defun swap-vars-case (n m numvars)
+  `(logior (the (unsigned-byte ,(ash 1 numvars))
+                (logand ,(loghead (ash 1 numvars)
+                                  (logeqv (var m numvars)
+                                          (var n numvars)))
+                        (the (unsigned-byte ,(ash 1 numvars)) truth)))
+           (the (unsigned-byte ,(ash 1 numvars))
+                (ash (the (unsigned-byte ,(ash 1 numvars))
+                          (logand ,(logand (var n numvars)
+                                           (lognot (var m numvars)))
+                                  (the (unsigned-byte ,(ash 1 numvars)) truth)))
+                     ,(- (ash 1 m) (ash 1 n))))
+           (the (unsigned-byte ,(ash 1 numvars))
+                (ash (the (unsigned-byte ,(ash 1 numvars))
+                          (logand ,(logand (var m numvars)
+                                           (lognot (var n numvars)))
+                                  (the (unsigned-byte ,(ash 1 numvars)) truth)))
+                     ,(- (ash 1 n) (ash 1 m))))))
+
+(defun swap-vars-inner-loop (n m numvars)
+  (if (zp m)
+      nil
+    (cons (list (if (eql m 1) 'otherwise (1- m))
+                (swap-vars-case n (1- m) numvars))
+          (swap-vars-inner-loop n (1- m) numvars))))
+
+(defun swap-vars-outer-case (n numvars)
+  `(case m
+     . ,(swap-vars-inner-loop n n numvars)))
+
+(defun swap-vars-outer-loop (n numvars)
+  (if (or (zp n) (<= n 2))
+      `((otherwise ,(swap-vars-case 1 0 numvars)))
+    (cons (list (1- n)
+                (swap-vars-outer-case (1- n) numvars))
+          (swap-vars-outer-loop (1- n) numvars))))
+
+(defmacro swap-vars-cases (numvars)
+  (if (eql numvars 2)
+      (swap-vars-case 1 0 numvars)
+    `(case n
+       . ,(swap-vars-outer-loop numvars numvars))))
+
+
+
+
+(local (defthmd logcdr-when-not-integerp
+         (implies (not (integerp x))
+                  (equal (logcdr x) 0))
+         :hints(("Goal" :in-theory (enable logcdr)))))
+(local (defthmd logcar-when-not-integerp
+         (implies (not (integerp x))
+                  (equal (logcar x) 0))
+         :hints(("Goal" :in-theory (enable logcar)))))
+
+(local
+ (encapsulate nil
+   (local (defun ind (width a b)
+            (if (zp width)
+                (list a b)
+              (ind (1- width) (logcdr a) (logcdr b)))))
+   (defthm logand-with-unsigned-byte
+     (implies (and (unsigned-byte-p width b)
+                   (syntaxp (and (quotep a)
+                                 (quotep width)))
+                   (not (unsigned-byte-p width a)))
+              (equal (logand a b)
+                     (logand (loghead width a) b)))
+     :hints (("goal" :induct (ind width a b)
+              :in-theory (enable* ihsext-recursive-redefs
+                                  logcar-when-not-integerp
+                                  logcdr-when-not-integerp))))))
+
+(local (defthm unsigned-byte-p-of-1
+         (implies (posp m)
+                  (unsigned-byte-p m 1))
+         :hints(("Goal" :in-theory (enable unsigned-byte-p)))))
+
+(local (defthm ash-of-minus-1
+         (implies (natp n)
+                  (equal (ash -1 n)
+                         (- (ash 1 n))))
+         :hints(("Goal" :in-theory (enable* ihsext-inductions
+                                            ihsext-recursive-redefs
+                                            logcons)))))
+
+(local (defthm ash-by-bound
+         (implies (and (< n bound)
+                       (syntaxp (quotep bound))
+                       (natp bound)
+                       (integerp n)
+                       (<= (ash 1 (- bound 1)) m))
+                  (<= (ash 1 n) m))
+         :hints (("goal" :use ((:instance bitops::|(< (ash a b) (ash a c))|
+                                (a 1) (b (- bound 1)) (c n)))
+                  :in-theory (disable bitops::|(< (ash a b) (ash a c))|)))))
+
+(local (defthm ash-by-bound-neg
+         (implies (and (< n bound)
+                       (syntaxp (quotep bound))
+                       (natp bound)
+                       (integerp n)
+                       (<= m (- (ash 1 (- bound 1)))))
+                  (<= m (- (ash 1 n))))
+         :hints (("goal" :use ((:instance ash-by-bound (m (- m))))
+                  :in-theory (disable ash-by-bound)))))
+
+
+(local (defthm ash-1-n-positive
+         (implies (natp n)
+                  (posp (ash 1 n)))
+         :rule-classes :type-prescription))
+
+(local (defthm ash-of-logand
+         (equal (ash (logand a b) sh)
+                (logand (ash a sh) (ash b sh)))
+         :hints(("Goal" :in-theory (enable* ihsext-inductions
+                                            ihsext-recursive-redefs)))))
+
+(local
+ (defthm ash-1-monotonic
+   (implies (and (< a b)
+                 (natp a)
+                 (integerp b))
+            (< (ash 1 a)
+               (ash 1 b)))
+   :hints(("Goal" :in-theory (enable bitops::ash-is-expt-*-x)))
+   :rule-classes ((:rewrite) (:linear))))
+
+(local (defthm signed-byte-p-by-unsigned-byte-p
+         (implies (unsigned-byte-p (1- w) x)
+                  (signed-byte-p w x))
+         :hints(("Goal" :in-theory (enable unsigned-byte-p signed-byte-p)))))
+
+
+
+(local (in-theory (disable bitops::logior-<-0-linear-2
+                           bitops::logior-<-0-linear-1
+                           bitops::logand->=-0-linear-1
+                           bitops::upper-bound-of-logand
+                           bitops::|(< a (logtail n a))|
+                           acl2::natp-posp
+                           bitops::lognot-<-const
+                           acl2::posp-rw
+                           acl2::posp-redefinition
+                           acl2::ifix-when-not-integerp)))
+
 (progn
   (defconst *truth-defs*
     '(defsection truth<NUMVARS>
-       (local (include-book "centaur/bitops/ihsext-basics" :dir :system))
-       (local (include-book "centaur/bitops/signed-byte-p" :dir :system))
-       (local (include-book "centaur/bitops/ash-bounds" :dir :system))
-       (local (include-book "arithmetic/top-with-meta" :dir :system))
-       (local (include-book "std/basic/arith-equivs" :dir :system))
-       (local (in-theory (disable unsigned-byte-p signed-byte-p)))
-
+       
        (define true<NUMVARS> ()
          :inline t :enabled t
          (mbe :logic (truth-norm (true) <NUMVARS>)
@@ -103,39 +281,6 @@
          (mbe :logic (truth-norm truth <NUMVARS>)
               :exec (logand <MASK> truth)))
 
-       (local (defthm unsigned-byte-p-of-1
-                (implies (posp m)
-                         (unsigned-byte-p m 1))
-                :hints(("Goal" :in-theory (enable unsigned-byte-p)))))
-
-       (local (defthm ash-of-minus-1
-                (implies (natp n)
-                         (equal (ash -1 n)
-                                (- (ash 1 n))))
-                :hints(("Goal" :in-theory (enable* ihsext-inductions
-                                                   ihsext-recursive-redefs
-                                                   logcons)))))
-
-       (local (defthm ash-by-bound
-                (implies (and (< n bound)
-                              (syntaxp (quotep bound))
-                              (natp bound)
-                              (integerp n)
-                              (<= (ash 1 (- bound 1)) m))
-                         (<= (ash 1 n) m))
-                :hints (("goal" :use ((:instance bitops::|(< (ash a b) (ash a c))|
-                                       (a 1) (b (- bound 1)) (c n)))
-                         :in-theory (disable bitops::|(< (ash a b) (ash a c))|)))))
-
-       (local (defthm ash-by-bound-neg
-                (implies (and (< n bound)
-                              (syntaxp (quotep bound))
-                              (natp bound)
-                              (integerp n)
-                              (<= m (- (ash 1 (- bound 1)))))
-                         (<= m (- (ash 1 n))))
-                :hints (("goal" :use ((:instance ash-by-bound (m (- m))))
-                         :in-theory (disable ash-by-bound)))))
 
 
 
@@ -158,17 +303,13 @@
                                        (ash -1
                                             (the (integer 0 <NUMVARS-1>) (lnfix n))))))))))
 
-       (local (defthm ash-1-n-positive
-                (implies (natp n)
-                         (posp (ash 1 n)))
-                :rule-classes :type-prescription))
-
        (define negative-cofactor<NUMVARS> ((n :type (integer 0 <NUMVARS-1>))
                                            (truth :type (unsigned-byte <WIDTH>)))
          :guard (and (natp n) (< n <NUMVARS>)
                      (unsigned-byte-p <WIDTH> truth))
          :guard-hints (("goal" :in-theory (e/d (negative-cofactor)
-                                               (var-negated-masked-size))
+                                               (var-negated-masked-size
+                                                ash-of-logand))
                         :use ((:instance size-of-logand-by-size-of-loghead
                                (a truth) (b (lognot (var n <NUMVARS>)))
                                (m <WIDTH>) (n (- <WIDTH> (ash 1 (nfix n)))))
@@ -217,44 +358,99 @@
                          (lognot (the (unsigned-byte <WIDTH>)
                                       (negative-cofactor<NUMVARS> n truth))))))))
 
+       ;; Various swap-vars implementations benchmarked below -- enumerating
+       ;; all the cases seems fastest for up to 6 vars
        (define swap-vars<NUMVARS> ((n :type (integer 0 <NUMVARS-1>))
                                    (m :type (integer 0 <NUMVARS-1>))
                                    (truth :type (unsigned-byte <WIDTH>)))
          :guard (and (natp n) (< n <NUMVARS>)
-                     (natp m) (< m <NUMVARS>)
+                     (natp m) (< m n)
                      (unsigned-byte-p <WIDTH> truth))
-         :guard-hints (("goal" :in-theory (enable swap-vars)))
-         :enabled t
+         :guard-hints (("Goal" :in-theory (enable swap-vars)))
          :split-types t
+         :enabled t
          (mbe :logic (swap-vars n m truth <NUMVARS>)
-              :exec (b* (((the (unsigned-byte <WIDTH>) xn1)
-                          (the (unsigned-byte <WIDTH>)
-                               (positive-cofactor<NUMVARS>
-                                (the (integer 0 <NUMVARS-1>) n)
-                                (the (unsigned-byte <WIDTH>) truth))))
-                         ((the (unsigned-byte <WIDTH>) xn0) (negative-cofactor<NUMVARS> n truth))
-                         ((the (unsigned-byte <WIDTH>) xn1m1) (positive-cofactor<NUMVARS> m xn1))
-                         ((the (unsigned-byte <WIDTH>) xn1m0) (negative-cofactor<NUMVARS> m xn1))
-                         ((the (unsigned-byte <WIDTH>) xn0m1) (positive-cofactor<NUMVARS> m xn0))
-                         ((the (unsigned-byte <WIDTH>) xn0m0) (negative-cofactor<NUMVARS> m xn0))
-                         ((the (unsigned-byte <WIDTH>) mvar) (var<NUMVARS> m))
-                         ((the (unsigned-byte <WIDTH>) nvar) (var<NUMVARS> n))
-                         ((the (signed-byte <WIDTH+1>) ~mvar) (lognot mvar))
-                         ((the (signed-byte <WIDTH+1>) ~nvar) (lognot nvar))
-                         ;; want (if n (if m xn1m1 xn0m1) (if m xn1m0 xn0m0))
-                         ((the (unsigned-byte <WIDTH>) n1case)
-                          (the (unsigned-byte <WIDTH>)
-                               (logior (the (unsigned-byte <WIDTH>)
-                                            (logand (the (unsigned-byte <WIDTH>) mvar)
-                                                    (the (unsigned-byte <WIDTH>) xn1m1)))
-                                       (the (unsigned-byte <WIDTH>)
-                                            (logand (the (signed-byte <WIDTH+1>) ~mvar)
-                                                    (the (unsigned-byte <WIDTH>) xn0m1))))))
-                         ((the (unsigned-byte <WIDTH>) n0case)
-                          (logior (the (unsigned-byte <WIDTH>) (logand mvar xn1m0))
-                                  (the (unsigned-byte <WIDTH>) (logand ~mvar xn0m0)))))
-                      (logior (the (unsigned-byte <WIDTH>) (logand nvar n1case))
-                              (the (unsigned-byte <WIDTH>) (logand ~nvar n0case))))))))
+              :exec (swap-vars-cases <NUMVARS>)))
+
+       ;; very marginally faster for the adjacent variables case
+       (define swap-adjacent-vars<NUMVARS> ((m :type (integer 0 <NUMVARS-1>))
+                                   (truth :type (unsigned-byte <WIDTH>)))
+         :guard (and (natp m) (< m <NUMVARS-1>)
+                     (unsigned-byte-p <WIDTH> truth))
+         :guard-hints (("Goal" :in-theory (enable swap-vars)))
+         :split-types t
+         :enabled t
+         (mbe :logic (swap-vars (+ 1 (nfix m)) m truth <NUMVARS>)
+              :exec (swap-adjacent-cases <NUMVARS>)))
+
+       ;; (define swap-vars-old<NUMVARS> ((n :type (integer 0 <NUMVARS-1>))
+       ;;                             (m :type (integer 0 <NUMVARS-1>))
+       ;;                             (truth :type (unsigned-byte <WIDTH>)))
+       ;;   :guard (and (natp n) (< n <NUMVARS>)
+       ;;               (natp m) (< m <NUMVARS>)
+       ;;               (unsigned-byte-p <WIDTH> truth))
+       ;;   :guard-hints (("goal" :in-theory (enable swap-vars)))
+       ;;   :enabled t
+       ;;   :split-types t
+       ;;   ;; (mbe :logic (swap-vars n m truth <NUMVARS>)
+       ;;   (b* (((the (unsigned-byte <WIDTH>) xn1)
+       ;;         (the (unsigned-byte <WIDTH>)
+       ;;              (positive-cofactor<NUMVARS>
+       ;;               (the (integer 0 <NUMVARS-1>) n)
+       ;;               (the (unsigned-byte <WIDTH>) truth))))
+       ;;        ((the (unsigned-byte <WIDTH>) xn0) (negative-cofactor<NUMVARS> n truth))
+       ;;        ((the (unsigned-byte <WIDTH>) xn1m1) (positive-cofactor<NUMVARS> m xn1))
+       ;;        ((the (unsigned-byte <WIDTH>) xn1m0) (negative-cofactor<NUMVARS> m xn1))
+       ;;        ((the (unsigned-byte <WIDTH>) xn0m1) (positive-cofactor<NUMVARS> m xn0))
+       ;;        ((the (unsigned-byte <WIDTH>) xn0m0) (negative-cofactor<NUMVARS> m xn0))
+       ;;        ((the (unsigned-byte <WIDTH>) mvar) (var<NUMVARS> m))
+       ;;        ((the (unsigned-byte <WIDTH>) nvar) (var<NUMVARS> n))
+       ;;        ((the (signed-byte <WIDTH+1>) ~mvar) (lognot mvar))
+       ;;        ((the (signed-byte <WIDTH+1>) ~nvar) (lognot nvar))
+       ;;        ;; want (if n (if m xn1m1 xn0m1) (if m xn1m0 xn0m0))
+       ;;        ((the (unsigned-byte <WIDTH>) n1case)
+       ;;         (the (unsigned-byte <WIDTH>)
+       ;;              (logior (the (unsigned-byte <WIDTH>)
+       ;;                           (logand (the (unsigned-byte <WIDTH>) mvar)
+       ;;                                   (the (unsigned-byte <WIDTH>) xn1m1)))
+       ;;                      (the (unsigned-byte <WIDTH>)
+       ;;                           (logand (the (signed-byte <WIDTH+1>) ~mvar)
+       ;;                                   (the (unsigned-byte <WIDTH>) xn0m1))))))
+       ;;        ((the (unsigned-byte <WIDTH>) n0case)
+       ;;         (logior (the (unsigned-byte <WIDTH>) (logand mvar xn1m0))
+       ;;                 (the (unsigned-byte <WIDTH>) (logand ~mvar xn0m0)))))
+       ;;     (logior (the (unsigned-byte <WIDTH>) (logand nvar n1case))
+       ;;             (the (unsigned-byte <WIDTH>) (logand ~nvar n0case)))))
+
+
+       ;; (define swap-vars*<NUMVARS> ((n :type (integer 0 <NUMVARS-1>))
+       ;;                             (m :type (integer 0 <NUMVARS-1>))
+       ;;                             (truth :type (unsigned-byte <WIDTH>)))
+       ;;   :guard (and (natp n) (< n <NUMVARS>)
+       ;;               (natp m) (< m n)
+       ;;               (unsigned-byte-p <WIDTH> truth))
+       ;;   :guard-hints (("Goal" :in-theory (enable swap-vars)))
+       ;;   :split-types t
+       ;;   :enabled t
+       ;;   (mbe :logic (swap-vars n m truth <NUMVARS>)
+       ;;        :exec (b* (((the (unsigned-byte <WIDTH>) varn) (var<NUMVARS> n))
+       ;;                   ((the (unsigned-byte <WIDTH>) varm) (var<NUMVARS> m))
+       ;;                   ((the (signed-byte <WIDTH+1>) same) (logeqv varn varm))
+       ;;                   ((the (unsigned-byte <WIDTH>) n&~m) (logand varn (lognot varm)))
+       ;;                   ((the (unsigned-byte <WIDTH>) m&~n) (logand varm (lognot varn)))
+       ;;                   ((the (unsigned-byte <WIDTH>) shift)
+       ;;                    (- (the (unsigned-byte <WIDTH>) (ash 1 (lnfix n)))
+       ;;                       (the (unsigned-byte <WIDTH>) (ash 1 (lnfix m))))))
+       ;;                (logior (the (unsigned-byte <WIDTH>) (logand same truth))
+       ;;                        (the (unsigned-byte <WIDTH>)
+       ;;                             (ash (the (unsigned-byte <WIDTH>) (logand n&~m truth))
+       ;;                                  (- shift)))
+       ;;                        (the (unsigned-byte <WIDTH>)
+       ;;                             (ash (the (unsigned-byte <WIDTH>) (logand m&~n truth))
+       ;;                                  shift))))))
+
+
+       ))
 
   (defmacro deftruthsize (n)
     `(make-event
@@ -275,4 +471,107 @@
   (deftruthsize 4)
   (deftruthsize 3))
 
-                      
+
+#||
+
+;; 0.35 sec:
+(time
+ (loop for i from 1 to 10000000 do
+       (let ((truth (logand #xffff i)))
+         (loop for n from 1 to 3 do
+               (loop for m from 0 to (1- n) do
+                     (swap-vars4 n m truth))))))
+;; 2.6 sec:
+(time
+ (loop for i from 1 to 10000000 do
+       (let ((truth (logand #xffff i)))
+         (loop for n from 1 to 3 do
+               (loop for m from 0 to (1- n) do
+                     (swap-vars*4 n m truth))))))
+
+;; 1.4 sec:
+(time
+ (loop for i from 1 to 10000000 do
+       (let ((truth (logand #xffff i)))
+         (loop for n from 1 to 3 do
+               (loop for m from 0 to (1- n) do
+                     (swap-vars-old4 n m truth))))))
+
+;; 0.33 sec:
+(time
+ (loop for i from 1 to 10000000 do
+       (let ((truth (logand #xffff i)))
+         (loop for n from 1 to 3 do
+               (loop for m from 0 to (1- n) do
+                     (swap-adjacent-vars4 m truth))))))
+
+
+;; 0.59 sec:
+(time
+ (loop for i from 1 to 10000000 do
+       (let ((truth (* i 429)))
+         (loop for n from 1 to 4 do
+               (loop for m from 0 to (1- n) do
+                     (swap-vars5 n m truth))))))
+;; 4.3 sec:
+(time
+ (loop for i from 1 to 10000000 do
+       (let ((truth (* i 429)))
+         (loop for n from 1 to 4 do
+               (loop for m from 0 to (1- n) do
+                     (swap-vars*5 n m truth))))))
+
+;; 2.6 sec:
+(time
+ (loop for i from 1 to 10000000 do
+       (let ((truth (* i 429)))
+         (loop for n from 1 to 4 do
+               (loop for m from 0 to (1- n) do
+                     (swap-vars-old5 n m truth))))))
+
+;; 0.51 sec:
+(time
+ (loop for i from 1 to 10000000 do
+       (let ((truth (* i 429)))
+         (loop for n from 1 to 4 do
+               (loop for m from 0 to (1- n) do
+                     (swap-adjacent-vars4 m truth))))))
+
+
+
+;; 11.8 sec:
+(time
+ (loop for i from 1 to 10000000 do
+       (let ((truth (* i #x1AD7F29ABCA)))
+         (loop for n from 1 to 5 do
+               (loop for m from 0 to (1- n) do
+                     (swap-vars6 n m truth))))))
+
+;; 54.6 sec:
+(time
+ (loop for i from 1 to 10000000 do
+       (let ((truth (* i #x1AD7F29ABCA)))
+         (loop for n from 1 to 5 do
+               (loop for m from 0 to (1- n) do
+                     (swap-vars*6 n m truth))))))
+
+;; 124 sec:
+(time
+ (loop for i from 1 to 10000000 do
+       (let ((truth (* i #x1AD7F29ABCA)))
+         (loop for n from 1 to 5 do
+               (loop for m from 0 to (1- n) do
+                     (swap-vars-old6 n m truth))))))
+
+;; 13.3 sec:
+(time
+ (loop for i from 1 to 10000000 do
+       (let ((truth (* i #x1AD7F29ABCA)))
+         (loop for n from 1 to 5 do
+               (loop for m from 0 to (1- n) do
+                     (swap-adjacent-vars6 m truth))))))
+
+
+
+
+||#
